testing/Base64/lampe/deps/noir_base64-0.0.0/lampe/noir_base64-0.0.0/Extracted.lean
@@ -8,7 +8,7 @@ import «noir_base64-0.0.0».Extracted.Encoder.ToBeRadix
 import «noir_base64-0.0.0».Extracted.GeneratedTypes
 import «noir_base64-0.0.0».Extracted.Lib
 import «noir_base64-0.0.0».Extracted.Tables
-import «std-1.0.0-beta.14».Extracted
+import std.Extracted
 
 namespace «noir_base64-0.0.0»
 
@@ -19,4 +19,4 @@ def env := Benchmarks.Mod.env
   ++ Encoder.env
   ++ Lib.env
   ++ Tables.env
-  ++ «std-1.0.0-beta.14».env
+  ++ std.env
