stdlib/lampe/Stdlib/Collections/Map.lean
@@ -1,6 +1,6 @@
-import «std-1.0.0-beta.14».Extracted
+import std.Extracted
 import Lampe
 
 namespace Lampe.Stdlib.Collections.Map
 
-open «std-1.0.0-beta.14»
+open std
