stdlib/lampe/Stdlib/Field/Mod.lean
@@ -1,4 +1,4 @@
-import «std-1.0.0-beta.14».Extracted
+import std.Extracted
 import Lampe
 import Lampe.Data.Digits
 import Stdlib.Field.Basic
@@ -8,7 +8,7 @@ import Stdlib.Ext
 
 namespace Lampe.Stdlib.Field
 
-open «std-1.0.0-beta.14» (env)
+open std (env)
 
 lemma bits_lt_of_lex_lt {data pdata : List (BitVec 1)}
     (hlen : data.length = pdata.length)
@@ -75,7 +75,7 @@ lemma ofDigitsBE'_lt_of_shorter_than_modulus {r : Radix} {data : List (Digit r)}
 
 theorem to_be_radix_intro :
     STHoare p env ⟦⟧
-    («std-1.0.0-beta.14::field::to_be_radix».call h![N] h![f, 256])
+    («std::field::to_be_radix».call h![N] h![f, 256])
     fun o =>
       ∃∃ (v : List.Vector (Digit R256) N.toNat),
       o = v.map BitVec.ofFin ⋆
@@ -104,7 +104,7 @@ theorem to_be_radix_intro :
 
 theorem to_le_radix_intro :
     STHoare p env ⟦⟧
-    («std-1.0.0-beta.14::field::to_le_radix».call h![N] h![f, 256])
+    («std::field::to_le_radix».call h![N] h![f, 256])
     fun o =>
       ∃∃ (v : List.Vector (Digit R256) N.toNat),
       o = v.reverse.map BitVec.ofFin ⋆
@@ -132,7 +132,7 @@ theorem to_le_radix_intro :
 
 theorem to_be_bits_intro :
     STHoare p env ⟦⟧
-    («std-1.0.0-beta.14::field::to_be_bits».call h![N] h![f])
+    («std::field::to_be_bits».call h![N] h![f])
     fun r => ∃∃(lt : f.val < (2 ^ N.toNat)),
       r = (RadixVec.toDigitsBE (d := N.toNat) (r := 2)
         ⟨f.val, by simp_all [OfNat.ofNat]⟩ |>.map (BitVec.ofFin (w := 1))) := by
@@ -252,7 +252,7 @@ theorem to_be_bits_intro :
 set_option maxHeartbeats 300000
 theorem to_le_bits_intro :
     STHoare p env ⟦⟧
-    («std-1.0.0-beta.14::field::to_le_bits».call h![N] h![f])
+    («std::field::to_le_bits».call h![N] h![f])
     fun r => ∃∃(lt : f.val < (2 ^ N.toNat)),
       r = (RadixVec.toDigitsBE (d := N.toNat) (r := 2)
         ⟨f.val, by simp_all [OfNat.ofNat]⟩ |>.map (BitVec.ofFin (w := 1)) |>.reverse) := by
@@ -429,7 +429,7 @@ theorem to_le_bits_intro :
 
 theorem to_be_bytes_intro :
     STHoare p env ⟦⟧
-    («std-1.0.0-beta.14::field::to_be_bytes».call h![N] h![f])
+    («std::field::to_be_bytes».call h![N] h![f])
     fun o =>
       ∃∃(lt : f.val < (256 ^ N.toNat)), o = (RadixVec.toDigitsBE
         (d := N.toNat)
@@ -578,7 +578,7 @@ theorem to_be_bytes_intro :
 set_option maxHeartbeats 500000
 theorem to_le_bytes_intro :
     STHoare p env ⟦⟧
-    («std-1.0.0-beta.14::field::to_le_bytes».call h![N] h![f])
+    («std::field::to_le_bytes».call h![N] h![f])
     fun o =>
       ∃∃(lt : f.val < (256 ^ N.toNat)), o = (RadixVec.toDigitsBE
         (d := N.toNat)
@@ -744,7 +744,7 @@ theorem to_le_bytes_intro :
 set_option maxHeartbeats 2000000
 theorem pow_32_intro {p self exponent} :
     STHoare p env ⟦⟧
-      («std-1.0.0-beta.14::field::pow_32».call h![] h![self, exponent])
+      («std::field::pow_32».call h![] h![self, exponent])
       (fun r => ∃∃ hlt : exponent.val < 2^32, r = self ^ exponent.val) := by
   enter_decl
   steps [to_le_bits_intro]
@@ -923,7 +923,7 @@ theorem pow_32_intro {p self exponent} :
 
 theorem lt_intro {p self another} [Lampe.Crypto.Bn254.Prime p] :
     STHoare p env ⟦⟧
-      («std-1.0.0-beta.14::field::lt».call h![] h![self, another])
+      («std::field::lt».call h![] h![self, another])
       (fun r => r = decide (self.val < another.val)) := by
   enter_decl
   steps [Lampe.Stdlib.Compat.is_bn254_spec]
@@ -934,7 +934,7 @@ theorem lt_intro {p self another} [Lampe.Crypto.Bn254.Prime p] :
 
 theorem from_le_bytes_intro :
     STHoare p env ⟦⟧
-    («std-1.0.0-beta.14::field::from_le_bytes».call h![N] h![bytes])
+    («std::field::from_le_bytes».call h![N] h![bytes])
     fun output => output = Fp.ofBytesLE (P := p) bytes.toList := by
   rcases N with ⟨⟨N, hN⟩⟩
   enter_decl
@@ -962,7 +962,7 @@ theorem from_le_bytes_intro :
 
 theorem from_be_bytes_intro :
     STHoare p env ⟦⟧
-    («std-1.0.0-beta.14::field::from_be_bytes».call h![N] h![bytes])
+    («std::field::from_be_bytes».call h![N] h![bytes])
     fun output => output = Fp.ofBytesLE (P := p) bytes.toList.reverse := by
   rcases N with ⟨⟨N, hN⟩⟩
   enter_decl
@@ -992,7 +992,7 @@ theorem from_be_bytes_intro :
 
 theorem sgn0_intro :
     STHoare p env ⟦⟧
-    («std-1.0.0-beta.14::field::sgn0».call h![] h![f])
+    («std::field::sgn0».call h![] h![f])
     (fun r => r = @Builtin.CastTp.cast Tp.field (Tp.u 1) _ p f) := by
   enter_decl
   simpa using
@@ -1099,7 +1099,7 @@ private lemma ofBytesLE_split_eq_foldl {p} {bytes : List.Vector (BitVec 8) 32} :
 set_option maxRecDepth 4096 in
 theorem bytes32_to_field_spec {p bytes} :
     STHoare p env ⟦⟧
-      («std-1.0.0-beta.14::field::bytes32_to_field».call h![] h![bytes])
+      («std::field::bytes32_to_field».call h![] h![bytes])
       (fun r => r = (bytes.toList.zipIdx.foldl
         (fun (acc : Fp p) (ib : BitVec 8 × ℕ) =>
           acc + (ib.1.toNat : Fp p) * (256 : Fp p) ^ (31 - ib.2))
