stdlib/lampe/Stdlib/Stdlib.lean
@@ -1,5 +1,5 @@
-import «std-1.0.0-beta.14».Extracted
+import std.Extracted
 
 namespace Lampe.Stdlib
 
-export «std-1.0.0-beta.14» (env)
+export std (env)
