stdlib/lampe/Stdlib/String.lean
@@ -1,8 +1,8 @@
-import «std-1.0.0-beta.14».Extracted
+import std.Extracted
 import Lampe
 namespace Lampe.Stdlib.String
 
-open «std-1.0.0-beta.14»
+open std
 
 -- Note: the extraction returns `Slice<u8>` (= `List (U 8)`), not `Vec<u8>`.
 -- The Noir function `as_bytes_vec` returns `Vec<u8>`, but the Lampe extraction
@@ -12,7 +12,7 @@ set_option maxRecDepth 1500 in
 set_option linter.deprecated false in
 theorem as_bytes_vec_spec {p N self} :
     STHoare p env ⟦⟧
-      («std-1.0.0-beta.14::string::as_bytes_vec».call h![N] h![self])
+      («std::string::as_bytes_vec».call h![N] h![self])
       (fun r => r = self.toList) := by
   enter_decl
   steps
@@ -22,7 +22,7 @@ theorem as_bytes_vec_spec {p N self} :
 set_option maxRecDepth 1500 in
 theorem from_spec {p N a} :
     STHoare p env ⟦⟧
-      («std-1.0.0-beta.14::convert::From».from h![(Tp.u 8).array N] (.str N) h![] h![] h![a])
+      («std::convert::From».from h![(Tp.u 8).array N] (.str N) h![] h![] h![a])
       (fun r => r = Lampe.Builtin.arrayAsStr! a) := by
   resolve_trait
   steps
