stdlib/lampe/Stdlib/Vector.lean
@@ -1,10 +1,10 @@
-import «std-1.0.0-beta.14».Extracted
+import std.Extracted
 import Lampe
 import Stdlib.List
 import Stdlib.TraitMethods
 
 namespace Lampe.Stdlib.Vector
-open «std-1.0.0-beta.14»
+open std
 
 set_option maxRecDepth 2000
 
@@ -13,7 +13,7 @@ set_option Lampe.pp.STHoare true
 
 theorem append_spec {p T a b}
   : STHoare p env ⟦⟧
-    («std-1.0.0-beta.14::vector::append».call h![T] h![a, b])
+    («std::vector::append».call h![T] h![a, b])
     (fun r => r = a ++ b) := by
   enter_decl
   steps
@@ -33,7 +33,7 @@ theorem append_spec {p T a b}
 
 theorem as_array_spec {p T N input}
   : STHoare p env ⟦⟧
-    («std-1.0.0-beta.14::vector::as_array».call h![T, N] h![input])
+    («std::vector::as_array».call h![T, N] h![input])
     (fun r => r.toList = input) := by
   enter_decl
   steps
@@ -80,7 +80,7 @@ theorem map_spec {T U Env p f fb l}
         (fun r => Inv (ip ++ [e]) (rp ++ [r])))
   : STHoare p env
     (Inv [] [] ⋆ [λf ↦ fb])
-    («std-1.0.0-beta.14::vector::map».call h![T, U, Env] h![l, f])
+    («std::vector::map».call h![T, U, Env] h![l, f])
     (fun v => Inv l v ⋆ [λf ↦ fb]) := by
   enter_decl
   steps
@@ -110,7 +110,7 @@ theorem map_spec {T U Env p f fb l}
 theorem map_pure_spec {T U Env p f fb func l}
     (h_pure : ∀x, STHoare p env ⟦⟧ (fb h![x]) (fun r => r = func x))
   : STHoare p env [λf ↦ fb]
-    («std-1.0.0-beta.14::vector::map».call h![T, U, Env] h![l, f])
+    («std::vector::map».call h![T, U, Env] h![l, f])
     (fun v => v = l.map func) := by
   steps [map_spec (Inv := fun i o => o = i.map func)]
   · rfl
@@ -124,7 +124,7 @@ theorem mapi_spec {T U Env p f fb l}
         (fun r => inv (ip ++ [e]) (op ++ [r])))
   : STHoare p env
     (inv [] [] ⋆ [λf ↦ fb])
-    («std-1.0.0-beta.14::vector::mapi».call h![T, U, Env] h![l, f])
+    («std::vector::mapi».call h![T, U, Env] h![l, f])
     (fun v => inv l v ⋆ [λf ↦ fb]) := by
   enter_decl
   steps
@@ -169,7 +169,7 @@ theorem mapi_spec {T U Env p f fb l}
 theorem mapi_pure_spec {T U Env p f fb fEmb l}
     (inv_pure : ∀i x, (h : i < l.length) → STHoare p env ⟦⟧ (fb h![i, x]) (fun r => r = fEmb i x))
   : STHoare p env [λf ↦ fb]
-    («std-1.0.0-beta.14::vector::mapi».call h![T, U, Env] h![l, f])
+    («std::vector::mapi».call h![T, U, Env] h![l, f])
     (fun v => v = l.mapIdx fEmb) := by
   steps [mapi_spec (inv := fun i o => o = i.mapIdx fEmb)]
   · rfl
@@ -193,7 +193,7 @@ theorem for_each_spec {T Env p f fb l}
       ((lp ++ [e]) <+: l) → STHoare p env (Inv lp) (fb h![e]) (fun _ => Inv (lp ++ [e])))
   : STHoare p env
     (Inv [] ⋆ [λf ↦ fb])
-    («std-1.0.0-beta.14::vector::for_each».call h![T, Env] h![l, f])
+    («std::vector::for_each».call h![T, Env] h![l, f])
     (fun _ => Inv l ⋆ [λf ↦ fb]) := by
   enter_decl
   steps []
@@ -219,7 +219,7 @@ theorem for_eachi_spec {T Env p f fb l}
       ((ip ++ [e]) <+: l) → STHoare p env (inv ip) (fb h![ip.length, e]) (fun _ => inv (ip ++ [e])))
   : STHoare p env
     (inv [] ⋆ [λf ↦ fb])
-    («std-1.0.0-beta.14::vector::for_eachi».call h![T, Env] h![l, f])
+    («std::vector::for_eachi».call h![T, Env] h![l, f])
     (fun _ => inv l ⋆ [λf ↦ fb]) := by
   enter_decl
   steps
@@ -258,7 +258,7 @@ theorem fold_spec {p T U Env l a f fb}
         (fun r => inv (ip ++ [e]) r)))
   : STHoare p env
     (inv [] a ⋆ [λf ↦ fb])
-    («std-1.0.0-beta.14::vector::fold».call h![T, U, Env] h![l, a, f])
+    («std::vector::fold».call h![T, U, Env] h![l, a, f])
     (fun r => (inv l r) ⋆ [λf ↦ fb]) := by
   enter_decl
   steps
@@ -290,7 +290,7 @@ theorem fold_spec {p T U Env l a f fb}
 theorem fold_pure_spec {p T U Env l a f fb fEmb}
     (inv_pure : ∀a x, STHoare p env ⟦⟧ (fb h![a, x]) (fun r => r = fEmb a x))
   : STHoare p env [λf ↦ fb]
-    («std-1.0.0-beta.14::vector::fold».call h![T, U, Env] h![l, a, f])
+    («std::vector::fold».call h![T, U, Env] h![l, a, f])
     (fun r => r = l.foldl fEmb a ⋆ [λf ↦ fb]) := by
   steps [fold_spec (inv := fun xs v => v = xs.foldl fEmb a)]
   · rfl
@@ -305,7 +305,7 @@ theorem reduce_spec {p T Env l f fb}
         (fun r => inv (ip ++ [e]) r)))
   : STHoare p env
     ((inv [] l[0]) ⋆ [λf ↦ fb])
-    («std-1.0.0-beta.14::vector::reduce».call h![T, Env] h![l, f])
+    («std::vector::reduce».call h![T, Env] h![l, f])
     (fun r => (inv l.tail r) ⋆ [λf ↦ fb]) := by
   enter_decl
   steps
@@ -343,7 +343,7 @@ theorem reduce_pure_spec {p T Env l f fb fEmb}
     (l_len_gt : l.length > 0)
     (inv_pure : ∀a x, STHoare p env ⟦⟧ (fb h![a, x]) (fun r => r = fEmb a x))
   : STHoare p env [λf ↦ fb]
-    («std-1.0.0-beta.14::vector::reduce».call h![T, Env] h![l, f])
+    («std::vector::reduce».call h![T, Env] h![l, f])
     (fun r => r = l.tail.foldl fEmb l[0] ⋆ [λf ↦ fb]) := by
   steps [reduce_spec (inv := fun xs v => v = xs.foldl fEmb l[0])]
   · rfl
@@ -359,7 +359,7 @@ theorem filter_spec {p T Env l f fb}
         (fun r => inv (ip ++ [e]) (if r then (op ++ [e]) else op))))
   : STHoare p env
     (inv [] [] ⋆ [λf ↦ fb])
-    («std-1.0.0-beta.14::vector::filter».call h![T, Env] h![l, f])
+    («std::vector::filter».call h![T, Env] h![l, f])
     (fun r => (inv l r) ⋆ [λf ↦ fb]) := by
   enter_decl
   steps
@@ -400,7 +400,7 @@ theorem filter_spec {p T Env l f fb}
 theorem filter_pure_spec {p T Env l f fb fEmb}
     (inv_pure : ∀x, STHoare p env ⟦⟧ (fb h![x]) (fun r => r = fEmb x))
   : STHoare p env [λf ↦ fb]
-    («std-1.0.0-beta.14::vector::filter».call h![T, Env] h![l, f])
+    («std::vector::filter».call h![T, Env] h![l, f])
     (fun r => (r = l.filter fEmb)) := by
   steps [filter_spec (inv := fun xs v => v = xs.filter fEmb)]
   · rfl
@@ -419,7 +419,7 @@ theorem join_spec {p T a s}
     (t_app_sem : ∀a b, STHoare p env ⟦⟧ (Append.append h![] T h![] h![] h![a, b])
       (fun r => r = t_app_emb a b))
   : STHoare p env ⟦⟧
-    («std-1.0.0-beta.14::vector::join».call h![T] h![a, s])
+    («std::vector::join».call h![T] h![a, s])
     (fun r => r = if h : a.length > 0 then
       a.tail.foldl (fun l r => t_app_emb (t_app_emb l s) r) a[0]
     else t_empty_emb) := by
@@ -491,7 +491,7 @@ theorem all_spec {p T Env l f fb}
       (ip ++ [e] <+: l) → STHoare p env (inv ip op) (fb h![e]) (fun r => inv (ip ++ [e]) (op ∧ r)))
   : STHoare p env
     ((inv [] true) ⋆ [λf ↦ fb])
-    («std-1.0.0-beta.14::vector::all».call h![T, Env] h![l, f])
+    («std::vector::all».call h![T, Env] h![l, f])
     (fun r => (inv l r) ⋆ [λf ↦ fb]) := by
   enter_decl
   steps
@@ -528,7 +528,7 @@ theorem all_spec {p T Env l f fb}
 theorem all_pure_spec {p T Env l f fb fEmb}
     (inv_pure : ∀a, STHoare p env ⟦⟧ (fb h![a]) (fun r => r = fEmb a))
   : STHoare p env [λf ↦ fb]
-    («std-1.0.0-beta.14::vector::all».call h![T, Env] h![l, f])
+    («std::vector::all».call h![T, Env] h![l, f])
     (fun r => r = l.all fEmb) := by
   steps [all_spec (inv := fun x r => r = x.all fEmb)]
   · simp
@@ -545,7 +545,7 @@ theorem any_spec {p T Env l f fb}
       (ip ++ [e] <+: l) → STHoare p env (inv ip op) (fb h![e]) (fun r => inv (ip ++ [e]) (op ∨ r)))
   : STHoare p env
     ((inv [] false) ⋆ [λf ↦ fb])
-    («std-1.0.0-beta.14::vector::any».call h![T, Env] h![l, f])
+    («std::vector::any».call h![T, Env] h![l, f])
     (fun r => (inv l r) ⋆ [λf ↦ fb]) := by
   enter_decl
   steps
@@ -582,7 +582,7 @@ theorem any_spec {p T Env l f fb}
 theorem any_pure_spec {p T Env l f fb fEmb}
     (inv_pure : ∀a, STHoare p env ⟦⟧ (fb h![a]) (fun r => r = fEmb a))
   : STHoare p env [λf ↦ fb]
-    («std-1.0.0-beta.14::vector::any».call h![T, Env] h![l, f])
+    («std::vector::any».call h![T, Env] h![l, f])
     (fun r => r = l.any fEmb) := by
   steps [any_spec (inv := fun x r => r = x.any fEmb)]
   · simp
