testing/Sort/lampe/deps/check_shuffle-0.0.0/lampe/check_shuffle-0.0.0/Extracted/Lib.lean
@@ -30,7 +30,7 @@ noir_def «check_shuffle-0.0.0»::check_shuffle<T: Type, N: u32>(lhs: Array<T, N
     let idx = (#_arrayIndex returning u32)(shuffle_indices, (#_cast returning u32)(i));
     let expected = (#_arrayIndex returning T)(rhs, (#_cast returning u32)(idx));
     let result = (#_arrayIndex returning T)(lhs, (#_cast returning u32)(i));
-    (#_assert returning Unit)(((T as «std-1.0.0-beta.14»::cmp::Eq<>)::eq<> as λ(T, T) -> bool)(expected, result));
+    (#_assert returning Unit)(((T as std::cmp::Eq<>)::eq<> as λ(T, T) -> bool)(expected, result));
     #_skip
   };
   #_skip
@@ -51,13 +51,13 @@ noir_def «check_shuffle-0.0.0»::get_shuffle_indices<T: Type, N: u32>(lhs: Arra
     let idx = (#_arrayIndex returning u32)(shuffle_indices, (#_cast returning u32)(i));
     let expected = (#_arrayIndex returning T)(rhs, (#_cast returning u32)(idx));
     let result = (#_arrayIndex returning T)(lhs, (#_cast returning u32)(i));
-    (#_assert returning Unit)(((T as «std-1.0.0-beta.14»::cmp::Eq<>)::eq<> as λ(T, T) -> bool)(expected, result));
+    (#_assert returning Unit)(((T as std::cmp::Eq<>)::eq<> as λ(T, T) -> bool)(expected, result));
     #_skip
   };
   shuffle_indices
 }
 
-noir_trait_impl[«check_shuffle-0.0.0».impl_432]<> «std-1.0.0-beta.14»::cmp::Eq<> for «check_shuffle-0.0.0»::test::CompoundStruct<> where [] := {
+noir_trait_impl[«check_shuffle-0.0.0».impl_432]<> std::cmp::Eq<> for «check_shuffle-0.0.0»::test::CompoundStruct<> where [] := {
   noir_def eq<>(self: «check_shuffle-0.0.0»::test::CompoundStruct<>, other: «check_shuffle-0.0.0»::test::CompoundStruct<>) -> bool := {
     (#_bAnd returning bool)((#_bAnd returning bool)((#_bEq returning bool)(self.0, other.0), (#_fEq returning bool)(self.1, other.1)), (#_uEq returning bool)(self.2, other.2))
   };
